Crypto.v
@@ -1,0 +1,42 @@
+From ITree Require Import ITree.
+Import ITreeNotations.
+
+Section Crypto.
+  Parameter BS: Set. (** ByteString *)
+  Parameter P: Set.  (** Principals *)
+
+  Inductive Msg := mkMsg (principal: P)(payload: BS).
+
+  (** effects *)
+
+  (** High-level network spec *)
+  Inductive Net: Type -> Type :=
+  | Recv: Net Msg (** blocking *)
+  | Send : Msg -> Net unit.
+
+  (** Ghost types *)
+  Inductive E (p: P): Type -> Type := Enc: forall t: Type, t -> E p t.
+  Inductive S (p: P): Type -> Type := Sign: forall t: Type, t -> S p t.
+  Inductive Pub (p: P): Type := mkPub: BS -> Pub p.
+  Inductive Priv (p: P): Type := mkPriv: BS -> Priv p.
+  Inductive Sym(p: P): Type := mkSym: BS -> Sym p.
+
+  (** High-level PKI lang *)
+  Inductive PKI: Type -> Type :=
+  | EncPub(p: P)(k: Pub p)(plain: BS): PKI (E p BS)
+  | DecPriv(p: P)(k: Priv p)(cipher: E p BS): PKI BS
+  | SignPriv(p: P)(k: Priv p)(plain: BS): PKI (S p BS)
+  | CheckPub(p: P)(k: Pub p)(signed: S p BS): PKI bool
+  | EncSym(p: P)(k: Sym p)(plain: BS): PKI (E p BS)
+  | DecSym(p: P)(k: Sym p)(cipher: E p BS): PKI BS.
+
+  Definition recv : itree Net Msg := embed Recv.
+  Definition send : Msg -> itree Net unit := embed Send.
+  Definition encrypt := embed EncPub.
+  Definition decrypt := embed DecPriv.
+  Definition sign := embed SignPriv.
+  Definition check := embed CheckPub.
+  Definition sencrypt := embed EncSym.
+  Definition sdecrypt := embed DecSym.
+
+End Crypto.
